Minterm.thy
@@ -12,34 +12,138 @@ imports
   Test_Formulae
 begin
 
-
 subsection {* Minterms Definition *}
 
-typedef ('var, 'addr, 'k::finite) minterm 
+typedef ('var, 'k::finite) minterm 
   = "{S. ((\<exists>!l\<in>S::('var, 'k::finite) literal set. \<exists>n. 
-          (equivalence (UNIV::'addr set) (to_sl_formula l) (ext_card_heap_superior_to n)))
+          (to_sl_formula l) = (ext_card_heap_superior_to n))
         \<and> (\<exists>!l\<in>S::('var, 'k::finite) literal set. \<exists>n. 
-          (equivalence (UNIV::'addr set) (to_sl_formula l) (not (ext_card_heap_superior_to n)))))}"
+          (to_sl_formula l) = (not (ext_card_heap_superior_to n))))}"
 proof
-  define x::"('var, 'k::finite) literal set" 
-    where "x = {to_literal (ext_card_heap_superior_to 0), 
-                to_literal (not (ext_card_heap_superior_to 0))}"
-  show "x \<in> {S. (\<exists>!l. l \<in> S \<and> (\<exists>n. equivalence UNIV (to_sl_formula l) (ext_card_heap_superior_to n))) 
-              \<and> (\<exists>!l. l \<in> S \<and> (\<exists>n. equivalence UNIV (to_sl_formula l) (not (ext_card_heap_superior_to n))))}"
-  proof
-    define l1::"('var, 'k::finite) literal" where "l1 = to_literal (ext_card_heap_superior_to 0)"
-    have "l1 \<in> x"
-      by (simp add: l1_def x_def) 
-    moreover have "equivalence UNIV (to_sl_formula l1) (ext_card_heap_superior_to 0)" unfolding l1_def
-      by (simp add: literals_def test_formulae.intros(3) to_sl_formula_to_literal)
-    define l2::"('var, 'k::finite) literal" where "l2 = to_literal (not (ext_card_heap_superior_to 0))"
-    moreover have "l2 \<in> x"
-      by (simp add: l2_def x_def)
-    moreover have "equivalence UNIV (to_sl_formula l2) (not (ext_card_heap_superior_to 0))" unfolding l2_def
-      by (simp add: literals_def test_formulae.intros(3) to_sl_formula_to_literal)
-    ultimately show "(\<exists>!l. l \<in> x \<and> (\<exists>n. equivalence UNIV (to_sl_formula l) (ext_card_heap_superior_to n))) 
-                   \<and> (\<exists>!l. l \<in> x \<and> (\<exists>n. equivalence UNIV (to_sl_formula l) (not (ext_card_heap_superior_to n))))"  
-      oops
+  define l1::"('var, 'k::finite) sl_formula" where "l1 = ext_card_heap_superior_to 0"
+  have "l1\<in> test_formulae" unfolding l1_def using test_formulae.simps by auto
+  define x::"('var, 'k::finite) literal set"
+    where "x = {to_literal l1, to_literal (not l1)}"
+  show "x \<in> {S. ((\<exists>!l\<in>S::('var, 'k::finite) literal set. \<exists>n. 
+            (to_sl_formula l) = (ext_card_heap_superior_to n))
+          \<and> (\<exists>!l\<in>S::('var, 'k::finite) literal set. \<exists>n. 
+            (to_sl_formula l) = (not (ext_card_heap_superior_to n))))}"
+  proof (intro CollectI conjI ex1I)
+    show "to_literal l1 \<in> x" by (simp add: l1_def x_def) 
+    show "\<exists>n. to_sl_formula (to_literal l1) = ext_card_heap_superior_to n"
+    proof
+      show "to_sl_formula (to_literal l1) = ext_card_heap_superior_to 0" using \<open>l1\<in> test_formulae\<close>
+        unfolding l1_def by simp     
+    qed
+    show "\<And>l. l \<in> x \<and> (\<exists>n. to_sl_formula l = ext_card_heap_superior_to n) \<Longrightarrow> l = to_literal l1"
+    proof -
+      fix l
+      assume lprop: "l \<in> x \<and> (\<exists>n. to_sl_formula l = ext_card_heap_superior_to n)"
+      hence "\<exists>n. to_sl_formula l = ext_card_heap_superior_to n" by simp
+      from this obtain n where ndef: "to_sl_formula l = ext_card_heap_superior_to n" by auto
+      have "l = to_literal l1 \<or> l = to_literal (not l1)" using lprop unfolding x_def by simp
+      moreover have "l\<noteq> to_literal (not l1)"
+      proof (rule ccontr)
+        assume "\<not> l \<noteq> to_literal (not l1)"
+        hence "l = to_literal (not l1)" by simp
+        hence "to_sl_formula l = (not l1)" by (simp add: \<open>l1 \<in> test_formulae\<close>)
+        hence "((ext_card_heap_superior_to n)::('var, 'k::finite) sl_formula) = not l1" using ndef by simp
+        also have "... = ((not (ext_card_heap_superior_to 0))::('var, 'k::finite) sl_formula)" using  l1_def by simp
+        finally have "((ext_card_heap_superior_to n)::('var, 'k::finite) sl_formula) = not (ext_card_heap_superior_to 0)" .
+        thus False 
+        proof (cases "n = \<infinity>")
+          case True
+          hence "ext_card_heap_superior_to n = sl_false" by simp
+          thus ?thesis using  sl_formula.distinct
+          proof -
+            show ?thesis
+              by (metis \<open>ext_card_heap_superior_to (n::enat) = not (ext_card_heap_superior_to (0::enat))\<close> 
+                  \<open>ext_card_heap_superior_to (n::enat) = sl_false\<close> sl_formula.distinct(22))
+          qed
+        next
+          case False
+          show ?thesis
+          proof (cases "n = 0")
+            case True
+            hence "ext_card_heap_superior_to n = sl_true"
+              by (simp add: enat_defs(1)) 
+            thus ?thesis
+            proof -
+              show ?thesis
+                by (metis \<open>ext_card_heap_superior_to n = not l1\<close> \<open>ext_card_heap_superior_to n = sl_true\<close> sl_formula.distinct(5))
+            qed
+          next
+            case False
+            hence "\<exists>m. n = Suc m" using \<open>n\<noteq> \<infinity>\<close> using list_decode.cases zero_enat_def by auto 
+            from this obtain m where "n = Suc m" by auto
+            hence "ext_card_heap_superior_to (n::enat) = sl_conj (ext_card_heap_superior_to (m)) (not sl_emp)"
+              by simp
+            thus ?thesis
+            proof -
+              show ?thesis
+                by (metis (no_types) \<open>ext_card_heap_superior_to (n::enat) = 
+                  sl_conj (ext_card_heap_superior_to (enat (m::nat))) (not sl_emp)\<close> 
+                    \<open>to_sl_formula (l::('var, 'k) literal) = not (l1::('var, 'k) sl_formula)\<close> ndef 
+                    sl_formula.distinct(57))
+            qed
+          qed
+        qed
+      qed
+      ultimately show "l = to_literal l1" by simp
+    qed
+    show "to_literal (not l1) \<in> x" by (simp add: l1_def x_def) 
+    show "\<exists>n. to_sl_formula (to_literal (not l1)) = not (ext_card_heap_superior_to n)"
+    proof
+      show "to_sl_formula (to_literal (not l1)) = not (ext_card_heap_superior_to 0)" using \<open>l1\<in> test_formulae\<close>
+        unfolding l1_def by simp     
+    qed
+    show "\<And>l. l \<in> x \<and> (\<exists>n. to_sl_formula l = not (ext_card_heap_superior_to n)) \<Longrightarrow> l = to_literal (not l1)"
+    proof -
+      fix l
+      assume lprop: "l \<in> x \<and> (\<exists>n. to_sl_formula l = not (ext_card_heap_superior_to n))"
+      hence "\<exists>n. to_sl_formula l = not (ext_card_heap_superior_to n)" by simp
+      from this obtain n where ndef: "to_sl_formula l = not (ext_card_heap_superior_to n)" by auto
+      have "l = to_literal l1 \<or> l = to_literal (not l1)" using lprop unfolding x_def by simp
+      moreover have "l\<noteq> to_literal (l1)"
+      proof (rule ccontr)
+        assume "\<not> l \<noteq> to_literal (l1)"
+        hence "l = to_literal (l1)" by simp
+        hence "to_sl_formula l = (l1)" by (simp add: \<open>l1 \<in> test_formulae\<close>)
+        hence "((not (ext_card_heap_superior_to n))::('var, 'k::finite) sl_formula) = l1" using ndef by simp
+        also have "... = (((ext_card_heap_superior_to 0))::('var, 'k::finite) sl_formula)" using  l1_def by simp
+        also have "... = (sl_true::('var, 'k::finite) sl_formula)" by (simp add: enat_defs)
+        finally have "((not (ext_card_heap_superior_to n))::('var, 'k::finite) sl_formula) = (sl_true)" .
+        thus False 
+        proof (cases "n = \<infinity>")
+          case True
+          hence "ext_card_heap_superior_to n = sl_false" by simp
+          hence "not (ext_card_heap_superior_to n) = not sl_false" by simp
+          thus ?thesis using  sl_formula.distinct \<open>not (ext_card_heap_superior_to n) = sl_true\<close> by simp
+        next
+          case False
+          show ?thesis
+          proof (cases "n = 0")
+            case True
+            hence "ext_card_heap_superior_to n = sl_true"
+              by (simp add: enat_defs(1)) 
+            hence "not (ext_card_heap_superior_to n) = not sl_true" by simp
+            thus ?thesis using sl_formula.distinct \<open>not (ext_card_heap_superior_to n) = sl_true\<close> by simp
+          next
+            case False
+            hence "\<exists>m. n = Suc m" using \<open>n\<noteq> \<infinity>\<close> using list_decode.cases zero_enat_def by auto 
+            from this obtain m where "n = Suc m" by auto
+            hence "ext_card_heap_superior_to (n::enat) = sl_conj (ext_card_heap_superior_to (m)) (not sl_emp)"
+              by simp
+            hence "not (ext_card_heap_superior_to n) = not (sl_conj (ext_card_heap_superior_to (m)) (not sl_emp))" by simp
+            thus ?thesis using sl_formula.distinct \<open>not (ext_card_heap_superior_to n) = sl_true\<close> by simp
+          qed
+        qed
+      qed
+      ultimately show "l = to_literal (not l1)" by simp
+    qed
+  qed
+qed
+      
 
 
 (*
@@ -52,6 +156,7 @@ definition e_minterm
 - si minterm \<Rightarrow> b
 - si a et b \<Rightarrow> mintern
 *)
+
 
 
 end
